src/Lustre/LCausality.v
@@ -1,13 +1,16 @@
+From Coq Require Import String.
 From Coq Require Import List.
 Import List.ListNotations.
 Open Scope list_scope.
 From Coq Require Import Permutation.
 From Coq Require Import Setoid Morphisms.
 
-From Velus Require Import Common.
+From compcert Require Import common.Errors.
+
+From Velus Require Import Common Environment.
 From Velus Require Import Operators.
 From Velus Require Import Clocks.
-
+From Velus Require Import CheckGraph.
 From Velus Require Import Lustre.LSyntax.
 
 (** * Lustre causality *)
@@ -153,6 +156,409 @@ Module Type LCAUSALITY
     induction eqs; intros Hf; auto.
     inv Hf. constructor; auto.
     destruct a. intros x Hex; eauto.
+  Qed.
+
+  Lemma Is_causal_move_to_input : forall inputs eqs xs,
+      Is_causal inputs eqs ->
+      Is_causal (xs++inputs) (remove_member (list_eq_dec ident_eq_dec) xs eqs).
+  Proof.
+    induction eqs; intros * Hcaus; simpl in *; auto.
+    destruct a as [xs' es']; simpl.
+    destruct (list_eq_dec _ _ _); subst.
+    - inv Hcaus; eauto.
+    - inv Hcaus.
+      constructor; simpl in *; auto.
+      intros ? Hex. apply H2 in Hex.
+      rewrite in_app_iff.
+      destruct Hex as [Hin|?]; auto.
+        unfold vars_defined in *. rewrite in_flat_map in *.
+        destruct Hin as [[xs'' es''] [Hin1 Hin2]]; simpl in *.
+        destruct (list_eq_dec ident_eq_dec xs xs''); subst; auto.
+        left. exists (xs'', es''); split; auto.
+        eapply remove_member_neq_In; auto.
+  Qed.
+
+  Corollary Is_causal_moves_to_input : forall inputs eqs xs,
+      Is_causal inputs eqs ->
+      Is_causal (xs++inputs) (remove_members (list_eq_dec ident_eq_dec) (map (fun x => [x]) xs) eqs).
+  Proof.
+    intros * Hcaus.
+    unfold remove_members.
+    rewrite <- fold_left_rev_right. eapply Is_causal_incl with (ins1 := (rev xs) ++ inputs).
+    rewrite <- Permutation_rev; reflexivity.
+    rewrite <- map_rev.
+    remember (rev xs) as xs'. clear Heqxs'.
+    induction xs'; simpl; auto.
+    rewrite cons_is_app. eapply Is_causal_move_to_input; eauto.
+  Qed.
+
+  (** ** Causality check *)
+
+  Fixpoint collect_free_left m (e : exp) : list ident :=
+    let collect_free_lefts := flat_map (collect_free_left m) in
+    match e with
+    | Econst _ => []
+    | Evar id (_, (ck, _)) => [m id]
+    | Eunop _ e (_, (ck, _)) => (collect_free_left m e)
+    | Ebinop _ e1 e2 (_, (ck, _)) => (collect_free_left m e1)++(collect_free_left m e2)
+    | Efby e0s es anns =>
+      (collect_free_lefts e0s)
+    | Ewhen es id _ (_, (ck, _)) =>
+      (m id)::(collect_free_lefts es)
+    | Emerge id ets efs (_, (ck, _)) =>
+      (m id)::(collect_free_lefts ets)++(collect_free_lefts efs)
+    | Eite e ets efs (_, (ck, _)) =>
+      (collect_free_left m e)++(collect_free_lefts ets)++(collect_free_lefts efs)
+    | Eapp _ es None _ =>
+      collect_free_lefts es
+    | Eapp _ es (Some r) _ =>
+      (collect_free_lefts es)++(collect_free_left m r)
+    end.
+
+  Definition collect_free_lefts m (es : list exp) : list positive :=
+    (flat_map (collect_free_left m) es).
+
+  Definition build_var_map' (eqs: list equation) : Env.t ident :=
+    Env.adds' (flat_map (fun eq => match (fst eq) with
+                                | [] => []
+                                | hd::tl => map (fun x => (x, hd)) tl
+                                end) eqs)
+              (@Env.empty ident).
+
+  Definition build_var_map (eqs : list equation) : (ident -> ident) :=
+    fun x => match Env.find x (build_var_map' eqs) with
+          | Some y => y
+          | None => x
+          end.
+
+  Definition build_graph (n : node) : Env.t (list positive) :=
+    let varmap := build_var_map (n_eqs n) in
+    Env.from_list ((map_filter (fun eq =>
+                                  let frees := collect_free_lefts varmap (snd eq) in
+                                  match (fst eq) with
+                                  | [] => None
+                                  | hd::_ => Some (hd, frees)
+                                  end) (n_eqs n))
+                     ++(map (fun '(x, _) => (x, [])) (n_in n))).
+    (* let inputenv := Env.adds (map fst (n_in n)) (map (fun _ => []) (n_in n)) (@Env.empty (list ident)) in *)
+    (* fold_left (fun env eq => *)
+    (*              let frees := collect_free_lefts varmap (snd eq) in *)
+    (*              match (fst eq) with *)
+    (*              | [] => env *)
+    (*              | hd::_ => Env.add hd frees env *)
+    (*              end) (n_eqs n) inputenv. *)
+
+  Definition check_node_causality (n : node) :=
+    if check_graph (build_graph n)
+    then Errors.OK tt
+    else Errors.Error (MSG "Causality error in node '" :: CTX (n_name n) :: msg "'").
+
+  Definition check_causality (G : global) :=
+    mmap check_node_causality G.
+
+  Fact build_var_map_InMembers {B} : forall eqs (ins : list (ident * B)) x m,
+      InMembers
+        x (map_filter
+             (fun eq : list ident * list exp =>
+                match fst eq with
+                | [] => None
+                | hd :: _ => Some (hd, collect_free_lefts m (snd eq))
+                end) eqs ++ List.map (fun '(x0, _) => (x0, [])) ins) ->
+      In x (vars_defined eqs ++ map fst ins).
+  Proof.
+    intros * Hin.
+    rewrite fst_InMembers, in_map_iff in Hin.
+    destruct Hin as [[? ?] [? Hin]]; subst; simpl.
+    rewrite in_app_iff in *. destruct Hin as [Hin|Hin].
+    + left. eapply map_filter_In' in Hin as [[? ?] [? ?]]; simpl in *.
+      destruct l0; inv H0.
+      unfold vars_defined. rewrite in_flat_map. exists (i::l0, l1); simpl; auto.
+    + right. rewrite in_map_iff in *. destruct Hin as [[x ?] [Hs Hin]]; inv Hs.
+      exists (i, b); auto.
+  Qed.
+
+
+  Fact build_var_map_NoDupMembers {B} : forall eqs (ins : list (ident * B)) m,
+      NoDup (vars_defined eqs ++ map fst ins) ->
+      NoDupMembers
+        (map_filter
+           (fun eq : list ident * list exp =>
+              match fst eq with
+              | [] => None
+              | hd :: _ => Some (hd, collect_free_lefts m (snd eq))
+              end) eqs ++ List.map (fun '(x0, _) => (x0, [])) ins).
+  Proof.
+    induction eqs; intros * Hnd; simpl in *.
+    + rewrite fst_NoDupMembers, map_map.
+      erewrite map_ext; eauto. intros [? ?]; auto.
+    + destruct a as [xs es]; simpl in *.
+      rewrite <- app_assoc in Hnd.
+      destruct xs; simpl; auto.
+      constructor; auto.
+      2:apply NoDup_app_r in Hnd; eauto.
+      inv Hnd. apply not_In_app in H1 as [_ Hnin].
+      intros Hin.
+      eapply build_var_map_InMembers in Hin; auto.
+  Qed.
+
+  Lemma build_graph_dom : forall n xs,
+      Forall2 (fun x eq => exists tl, fst eq = x::tl) xs (n_eqs n) ->
+      Env.dom (build_graph n) (xs++(map fst (n_in n))).
+  Proof.
+    intros n. unfold build_graph.
+    generalize (build_var_map (n_eqs n)) as map.
+    specialize (in_vars_defined_NoDup n) as Hndup.
+    destruct n; simpl in *; clear - n_nodup0 Hndup.
+    assert (List.map fst (List.map (fun '(x, _) => (x, (@nil positive))) n_in0) = List.map fst n_in0) as Hfst.
+    { rewrite map_map. apply map_ext.
+      intros [? ?]; auto. }
+    induction n_eqs0; intros * Hf; simpl in *.
+    - inv Hf; simpl.
+      eapply Env.dom_from_list_map_fst; auto.
+      eapply NoDupMembers_app_l in n_nodup0.
+      rewrite fst_NoDupMembers in n_nodup0. rewrite fst_NoDupMembers, Hfst; auto.
+    - inv Hf. destruct H2 as [tl ?]. rewrite H; simpl.
+      unfold Env.from_list in *. rewrite Env.adds'_cons.
+      2:{ rewrite Permutation_swap, H in Hndup; simpl in Hndup.
+          intro contra.
+          eapply build_var_map_InMembers in contra.
+          inv Hndup. apply not_In_app in H2 as [_ Hnin].
+          apply Hnin. rewrite Permutation_app_comm; auto. }
+      apply Env.dom_add_cons; auto.
+      eapply IHn_eqs0; eauto.
+      + unfold anon_in_eqs in n_nodup0; simpl in n_nodup0.
+        rewrite (Permutation_app_comm (anon_in_eq _)) in n_nodup0.
+        repeat rewrite app_assoc in *. apply NoDupMembers_app_l in n_nodup0; auto.
+      + rewrite Permutation_swap in Hndup. apply NoDup_app_r in Hndup; auto.
+  Qed.
+
+  Lemma build_graph_find' : forall n x xs es,
+      In (x::xs, es) (n_eqs n) ->
+      Env.find x (build_graph n) = Some (collect_free_lefts (build_var_map (n_eqs n)) es).
+  Proof.
+    intros * Hin.
+    unfold build_graph.
+    eapply Env.find_In_from_list.
+    2:{ clear - n.
+        specialize (in_vars_defined_NoDup n) as Hndup.
+        remember (n_in n) as ins. remember (n_eqs n) as eqs. clear - Hndup.
+        rewrite Permutation_app_comm in Hndup.
+        eapply build_var_map_NoDupMembers; eauto. }
+    rewrite in_app_iff. left.
+    eapply map_filter_In; eauto.
+  Qed.
+
+  Fact collect_free_left_complete : forall m e x,
+      Is_free_left x e ->
+      In (m x) (collect_free_left m e).
+  Proof.
+    induction e using exp_ind2; intros * Hfree; inv Hfree; simpl;
+      try destruct a as [ty [ck name]];
+      simpl; repeat rewrite in_app_iff.
+    Local Ltac Forall_Exists_Exists H :=
+        eapply Forall_Exists in H; [|eauto];
+        rewrite in_flat_map';
+        eapply Exists_Exists; [|eauto]; intros ? [? ?]; auto.
+    - (* var *)
+      left; auto.
+    - (* unop *) auto.
+    - (* binop *) destruct H0; auto.
+    - (* fby *)
+      Forall_Exists_Exists H2.
+    - (* when *)
+      destruct H1 as [Hex|Hex].
+      + inv Hex. left; auto.
+      + right. Forall_Exists_Exists Hex.
+    - (* merge *)
+      destruct H2 as [Hex|[Hex|Hex]].
+      + inv Hex. left; auto.
+      + right; left. Forall_Exists_Exists Hex.
+      + right; right. Forall_Exists_Exists Hex.
+    - (* ite *)
+      destruct H2 as [Hex|[Hex|Hex]]; auto.
+      + right; left. Forall_Exists_Exists Hex.
+      + right; right. Forall_Exists_Exists Hex.
+    - (* app *)
+      Forall_Exists_Exists H2.
+    - (* app (reset) *)
+      inv H2; auto.
+      left. Forall_Exists_Exists H3.
+  Qed.
+
+  Corollary collect_free_lefts_complete : forall m es x,
+      Exists (Is_free_left x) es ->
+      In (m x) (collect_free_lefts m es).
+  Proof.
+    intros * Hex.
+    unfold collect_free_lefts. rewrite in_flat_map.
+    eapply Exists_exists in Hex as [e [Hin Hfree]].
+    exists e; split; auto.
+    eapply collect_free_left_complete in Hfree; eauto.
+  Qed.
+
+  Lemma build_graph_find : forall n,
+      Forall (fun '(xs, es) => forall x tl used,
+                  xs = x::tl ->
+                  Env.find x (build_graph n) = Some used ->
+                  (forall x, Exists (Is_free_left x) es -> In (build_var_map (n_eqs n) x) used))
+        ((map (fun '(x, _) => ([x], [])) (n_in n))++n_eqs n).
+  Proof.
+    intros n.
+    apply Forall_app; split.
+    - rewrite Forall_map.
+      eapply Forall_forall. intros [? [? ?]] Hin * Heq Hfind ? Hex. inv Hex.
+    - eapply Forall_forall. intros [? ?] Hin * ? Hfind ? Heqx; subst.
+      eapply build_graph_find' in Hin.
+      rewrite Hin in Hfind. inv Hfind.
+      eapply collect_free_lefts_complete; eauto.
+  Qed.
+
+  Fact build_var_map_incl1 : forall eqs,
+      forall x y, Env.find x (build_var_map' eqs) = Some y ->
+             Exists (fun eq => In x (fst eq) /\ In y (fst eq)) eqs.
+  Proof.
+    induction eqs; intros * Hfind;
+      unfold build_var_map' in Hfind; simpl in *.
+    - rewrite Env.gempty in Hfind; congruence.
+    - destruct a as [[|? xs] es]; simpl in Hfind. 1:right; eauto.
+      rewrite <- Env.adds'_app in Hfind.
+      eapply Env.find_adds'_In in Hfind as [Hin|Hfind]; eauto.
+      + right. apply in_flat_map in Hin as [[xs' es'] [Hin1 Hin2]]; simpl.
+        eapply Exists_exists. exists (xs', es'); split; auto; simpl in *.
+        destruct xs'. inv Hin2.
+        apply in_map_iff in Hin2 as [? [Hs Hin]]; inv Hs.
+        simpl; auto.
+      + eapply Env.find_adds'_In in Hfind as [Hin|Hfind].
+        * left.
+          apply in_map_iff in Hin as [? [Hs Hin]]; inv Hs.
+          simpl; auto.
+        * rewrite Env.gempty in Hfind; congruence.
+  Qed.
+
+  Lemma NoDup_vars_defined : forall eqs xs1 xs2 es1 es2 x,
+      NoDup (vars_defined eqs) ->
+      In (xs1, es1) eqs ->
+      In (xs2, es2) eqs ->
+      In x xs1 ->
+      In x xs2 ->
+      xs1 = xs2.
+  Proof.
+    induction eqs; intros * Hnd Hin1 Hin2 Hin3 Hin4.
+    - inv Hin1.
+    - inv Hin1; inv Hin2; auto; simpl in *. 2-3:exfalso.
+      + inv H; auto.
+      + eapply NoDup_app_In in Hnd; eauto.
+        eapply Hnd. unfold vars_defined. rewrite in_flat_map. exists (xs2, es2); auto.
+      + eapply NoDup_app_In in Hnd; eauto.
+        eapply Hnd. unfold vars_defined. rewrite in_flat_map. exists (xs1, es1); auto.
+      + eapply IHeqs; eauto. apply NoDup_app_r in Hnd; auto.
+  Qed.
+
+  Lemma build_var_map_incl2 : forall eqs,
+      NoDup (vars_defined eqs) ->
+      Forall (fun eq => forall x, In x (fst eq) <-> In (build_var_map eqs x) (fst eq)) eqs.
+  Proof.
+    intros eqs Hndup. unfold build_var_map.
+    specialize (build_var_map_incl1 eqs) as Hf.
+    eapply Forall_forall. intros [? ?] Hin1 ?; split; intros Hin2; simpl in *.
+    - destruct (Env.find x _) eqn:Hfind; auto.
+      eapply Hf, Exists_exists in Hfind as [[xs es] [Hi [Hi1 Hi2]]]; simpl in *.
+      eapply NoDup_vars_defined in Hin2; eauto. inv Hin2; auto.
+    - destruct (Env.find x _) eqn:Hfind; auto.
+      eapply Hf, Exists_exists in Hfind as [[xs es] [Hi [Hi1 Hi2]]]; simpl in *.
+      eapply NoDup_vars_defined in Hin2; eauto. inv Hin2; auto.
+  Qed.
+
+  Corollary build_var_map_vars_defined : forall eqs x,
+      NoDup (vars_defined eqs) ->
+      In x (vars_defined eqs) <-> In (build_var_map eqs x) (vars_defined eqs).
+  Proof.
+    intros * Hndup.
+    eapply build_var_map_incl2 in Hndup.
+    unfold vars_defined. repeat rewrite in_flat_map.
+    split; intros [eq [Hin1 Hin2]];
+      exists eq; split; auto;
+      eapply Forall_forall in Hin1; eauto; simpl in Hin1.
+    - rewrite <- Hin1; auto.
+    - rewrite Hin1; auto.
+  Qed.
+
+  Fact build_var_map_id : forall eqs x,
+      ~In x (vars_defined eqs) ->
+      (build_var_map eqs x) = x.
+  Proof.
+    intros * Hnin.
+    unfold build_var_map, build_var_map'.
+    rewrite Env.gsso', Env.gempty; auto.
+    rewrite fst_InMembers.
+    intro contra; apply Hnin; clear Hnin.
+    apply in_map_iff in contra as [[x' y] [? Hin]]; simpl in *; subst.
+    unfold vars_defined.
+    rewrite in_flat_map in *. destruct Hin as [[xs es] [Hin1 Hin2]].
+    exists (xs, es); split; simpl in *; auto.
+    destruct xs. inv Hin2.
+    apply in_map_iff in Hin2 as [? [Hs ?]]; inv Hs.
+    right; auto.
+  Qed.
+
+  Lemma build_var_map_incl : forall n,
+      Forall (fun eq => forall x, In (build_var_map (n_eqs n) x) (fst eq) -> In x (fst eq))
+             (n_eqs n ++ map (fun '(x, _) => ([x], [])) (n_in n)).
+  Proof.
+    intros n.
+    specialize (in_vars_defined_NoDup n) as Hndup.
+    eapply Forall_app; split.
+    - apply NoDup_app_r in Hndup; auto.
+      eapply build_var_map_incl2 in Hndup.
+      eapply Forall_impl; eauto. intros; simpl in *. rewrite H; auto.
+    - rewrite Forall_map. eapply Forall_forall. intros [? [? ?]] Hin ? Hin'; simpl in *.
+      destruct Hin' as [Hin'|?]; auto.
+      rewrite build_var_map_id in Hin'; auto.
+      intro contra; subst.
+      rewrite build_var_map_vars_defined in contra. 2:apply NoDup_app_r in Hndup; auto.
+      eapply NoDup_app_In in Hndup; eauto.
+      rewrite in_map_iff. eexists; split; eauto. auto.
+  Qed.
+
+  Fact m_vars_defined : forall m x eqs,
+      Forall (fun eq => forall x, In (m x) (fst eq) -> In x (fst eq)) eqs ->
+      In (m x) (vars_defined eqs) ->
+      In x (vars_defined eqs).
+  Proof.
+    induction eqs; intros Hf Hin; simpl in *; try inv Hin.
+    rewrite in_app_iff in *.
+    inv Hf.
+    destruct Hin as [Hin|?]; auto.
+  Qed.
+
+  Fact WellOrdered_Is_causal : forall graph m eqs xs,
+      Forall2 (fun x equ => exists tl, fst equ = x::tl) xs eqs ->
+      Forall (fun eq => forall x, In (m x) (fst eq) -> In x (fst eq)) eqs ->
+      Forall (fun '(xs, es) => forall hd tl used,
+                  xs = hd::tl ->
+                  Env.find hd graph = Some used ->
+                  (forall x, Exists (Is_free_left x) es -> In (m x) used)
+             ) eqs ->
+      WellOrdered graph xs ->
+      Is_causal [] eqs.
+  Proof.
+    induction eqs; intros * Heq Hm Hf Hord; simpl in *; auto.
+    destruct a as [xs' es]; simpl in *.
+    inv Heq. inv Hm. inv Hf. inv Hord.
+    constructor; simpl in *; eauto.
+    intros ? Hex. left.
+    destruct H2 as [tl ?]; subst.
+    specialize (H5 _ _ _ eq_refl H7).
+    apply H5, H8 in Hex.
+    clear - Hex H3 H4.
+    assert (In (m x0) (vars_defined eqs)) as Hin.
+    { eapply Forall2_forall2 in H3 as [Hlen ?].
+      eapply In_nth with (d:=x0) in Hex as [n [Hn Hnth]].
+      specialize (H _ ([], []) _ _ _ Hn Hnth eq_refl) as [tl' Hnth2].
+      setoid_rewrite Hlen in Hn. specialize (@nth_In _ n eqs ([], []) Hn) as Hin.
+      destruct (nth n eqs _) as [xs' es']; simpl in Hnth2.
+      unfold vars_defined. rewrite in_flat_map. exists (xs', es'); subst; simpl; split; auto. }
+    eapply m_vars_defined; eauto.
   Qed.
 
 End LCAUSALITY.
