src/Transcription/Transcription.v
@@ -22,7 +22,7 @@ Module Type TRANSCRIPTION
   Declare Module Export Typing : TRTYPING Ids Op OpAux L.Syn L.Typ L.Norm.Norm.Untuple CE.Syn CE.Typ NL.Syn NL.Ord NL.Typ Tr.
   Declare Module Export Clocking : TRCLOCKING Ids Op OpAux L.Syn L.Clo CE.Syn NL.Syn NL.Ord NL.Mem NL.IsD CE.IsF NL.IsF CE.Clo NL.Clo Tr.
   Declare Module Export Correctness : CORRECTNESS Ids Op OpAux L.Syn CE.Syn NL.Syn Tr L.Typ L.Clo L.Cau NL.Ord L.Ord CStr L.Sem L.ClSem NL.CoindSem.
-  Declare Module Export Completeness : COMPLETENESS Ids Op OpAux CStr L.Syn L.Norm.Norm CE.Syn NL.Syn Tr.
+  Declare Module Export Completeness : COMPLETENESS Ids Op OpAux CStr L.Syn L.Cau L.Norm.Norm CE.Syn NL.Syn Tr.
 End TRANSCRIPTION.
 
 Module TranscriptionFun
@@ -39,5 +39,5 @@ Module TranscriptionFun
   Module Export Typing := TrTypingFun Ids Op OpAux L.Syn L.Typ L.Norm.Norm.Untuple CE.Syn CE.Typ NL.Syn NL.Ord NL.Typ Tr.
   Module Export Clocking := TrClockingFun Ids Op OpAux L.Syn L.Clo CE.Syn NL.Syn NL.Ord NL.Mem NL.IsD CE.IsF NL.IsF CE.Clo NL.Clo Tr.
   Module Export Correctness := CorrectnessFun Ids Op OpAux L.Syn CE.Syn NL.Syn Tr L.Typ L.Clo L.Cau NL.Ord L.Ord CStr L.Sem L.ClSem NL.CoindSem.
-  Module Export Completeness := CompletenessFun Ids Op OpAux CStr L.Syn L.Norm.Norm CE.Syn NL.Syn Tr.
+  Module Export Completeness := CompletenessFun Ids Op OpAux CStr L.Syn L.Cau L.Norm.Norm CE.Syn NL.Syn Tr.
 End TranscriptionFun.
